feat: Sha3.updateLock

fstar/Zen.Sha3.Extracted.fst
@@ -7,6 +7,7 @@ open Zen.Types
 module Sha3 = Zen.Sha3.Realized
 module PK = Zen.PublicKey
 module A = Zen.Array
+module U32 = FStar.UInt32
 
 val updateCPK: PK.cpk -> Sha3.t -> Sha3.t `cost` 205
 let updateCPK (parity, h) s =
@@ -23,6 +24,83 @@ let updateContractId (v, h) sha3 =
     >>= Sha3.updateU32 v
     >>= Sha3.updateHash h
     end
+
+val lockId : lock -> U32.t `cost` 17
+let lockId lock =
+  begin match lock with
+  | FeeLock                  -> U32.uint_to_t 1
+  | PKLock _                 -> U32.uint_to_t 2
+  | ActivationSacrificeLock  -> U32.uint_to_t 3
+  | ContractLock _           -> U32.uint_to_t 4
+  | ExtensionSacrificeLock _ -> U32.uint_to_t 5
+  | CoinbaseLock _           -> U32.uint_to_t 6
+  | DestroyLock              -> U32.uint_to_t 7
+  | HighVLock (lid , _)      -> lid
+  end
+  |> incRet 17
+
+// WARNING: doesn't update HighV locks!
+val updateLock :
+  (lock:lock)
+  -> Sha3.t
+  -> Sha3.t `cost` 293
+let updateLock lock sha3 =
+  let! lid = lockId lock in // 17
+  match lock with
+  | PKLock hash ->
+      inc (31 + 29)
+      begin
+      ret sha3
+      >>= Sha3.updateU32 lid // 24
+      >>= Sha3.updateHash hash // 192
+      end
+  | ContractLock contractId ->
+      inc 29
+      begin
+      ret sha3
+      >>= Sha3.updateU32 lid // 24
+      >>= updateContractId contractId // 223
+      end
+  | FeeLock ->
+      inc (223 + 29)
+      begin
+      ret sha3
+      >>= Sha3.updateU32 lid // 24
+      end
+  | DestroyLock ->
+      inc (223 + 29)
+      begin
+      ret sha3
+      >>= Sha3.updateU32 lid // 24
+      end
+  | ActivationSacrificeLock ->
+      inc (223 + 29)
+      begin
+      ret sha3
+      >>= Sha3.updateU32 lid // 24
+      end
+  | ExtensionSacrificeLock contractId ->
+      inc 29
+      begin
+      ret sha3
+      >>= Sha3.updateU32 lid // 24
+      >>= updateContractId contractId // 223
+      end
+  | CoinbaseLock (blockNumber , hash) ->
+      inc (7 + 29)
+      begin
+      ret sha3
+      >>= Sha3.updateU32 lid // 24
+      >>= Sha3.updateU32 blockNumber  // 24
+      >>= Sha3.updateHash hash // 192
+      end
+  | HighVLock _ ->
+      // You can't update an High Version lock!
+      inc (247 + 29)
+      begin
+      ret sha3
+      end
+
 
 val updateListWith (#a : Type) (#n : nat) :
     (a -> Sha3.t -> Sha3.t `cost` n)
